proof/schnorr_protocol/W64_Zp_SchnorrIndistinguishability.ec
@@ -1,36 +1,48 @@
 require import AllCore Distr DInterval List Int IntDiv.
+require import AuxLemmas.
 
 from Jasmin require import JModel JBigNum.
 require import Array32 Array64 Array128.
-
-require import W64_SchnorrProtocol.
-require import Zp_SchnorrProtocol.
-require import AuxLemmas.
-
-require import Ring_ops_spec.
-import Zp DZmodP.
-import W64xN Sub R. 
-
-
 require import W64_SchnorrExtract.
-require import Ring_ops_proof.
+require import W64_SchnorrProtocol.
+
+
+require Constants.
+
+
+require import ModularMultiplication_Concrete.
+require import BarrettReduction_Concrete.
+
+require import Ring_ops_spec Ring_ops_proof.
+import W64xN R.                 
+(* import Sub  *)
+
+require Zp_SchnorrProtocol.
+
+
+clone import Zp_SchnorrProtocol as ZPSP with op q <= Constants.q,
+                                             op Zp.p <= Constants.p,
+                                             op g <= Zp.inzmod Constants.g,
+                                             type LSP.sbits <- sbits.
+import ZPSP.Zp Zp.DZmodP Zp.Sub.
 
 
 
+require MontgomeryLadder_Concrete.
+clone import MontgomeryLadder_Concrete as MLC with theory Zp <= Zp.
+
+axiom q_prime : prime q.
+axiom p_prime : prime p.
 
 
+axiom q_less_p       : q < p.
+axiom q_val_prop1 x  : W64xN.valR x < q * q. 
+axiom p_less_modulusR : p < W64xN.modulusR.
 
-axiom bn_set_gg_prop : 
-  phoare[ M.bn_set_g : true ==> valR res = Sub.val g  ] = 1%r.
-axiom bn_set_go_prop : 
-  phoare[ M.bn_set_p : true ==> valR res = p  ] = 1%r.
-axiom bn_set_bf_prop : 
-  phoare[ M.bn_set_bp : true ==> W64x2N.valR res = Ri  ] = 1%r.
-axiom bn_set_eo_prop : 
-  phoare[ M.bn_set_q : true ==> valR res = q  ] = 1%r.
-axiom bn_set_eb_prop : 
-  phoare[ M.bn_set_bq : true ==> W64x2N.valR res = Rip  ] = 1%r.
 
+op Rip : int = nasty_id (4 ^ (dnlimbs * nlimbs) %/ q).
+lemma Rip_def: Rip = 4 ^ (dnlimbs * nlimbs) %/ q.
+rewrite /Rip. smt(nasty_id). qed.
 
 
 lemma zp_eq z1 z2 : (val z1 = val z2) = (z1 = z2). smt(@Zp). qed.
@@ -40,11 +52,13 @@ lemma inzpKK: forall (z : int), val (inzmod z) = z %% p. smt(@Zp). qed.
 
   
 module ASpecFp_Schnorr = {
+
+
  proc commit(h : zmod, w : R) : zmod * int = {
    var r;
    var a : zmod;    
    r <@ ASpecFp.rsample(q);
-   a <@ ASpecFp.expm(g,r);
+   a <@ ML_Spec.expm(g,r);
    return (a,  r);
   } 
 
@@ -55,27 +69,12 @@ module ASpecFp_Schnorr = {
   }
 }.
 
-axiom q_less_p       : q < p.
-axiom q_val_prop1 x  : W64xN.valR x < q * q. 
-axiom p_less_modulusR : p < W64xN.modulusR.
-
-op g_int : int.
-
-op completeness_relationJ (s: W64xN.R.t) (w:W64xN.R.t) = g_int ^ (W64xN.valR w) %% p = W64xN.valR s %% p.
-op soundness_relationJ (s: W64xN.R.t) (w:W64xN.R.t) = g_int ^ (W64xN.valR w) %% p = W64xN.valR s %% p.
-
-
-
-
+op completeness_relationJ (s: W64xN.R.t) (w:W64xN.R.t) = Constants.g ^ (W64xN.valR w) %% p = W64xN.valR s %% p.
 
 lemma p_val_prop1 x : W64xN.valR x < p * p.  
 by smt(q_less_p q_val_prop1 q_prime prime_p). 
 qed.
 
-
-require import MontgomeryLadder_Concrete.
-require import ModularMultiplication_Concrete.
-require import BarrettReduction_Concrete.
 
 lemma xxx:
   forall (a b : int), (inzmod a) = (inzmod b) <=> a %% p = b %% p.
@@ -97,7 +96,7 @@ rewrite /ZModpField.exp. rewrite /ZModpRing.exp. auto. qed.
 
 
 lemma exps' (s : zmod) : forall n, 0 <= n => val (ZModpField.exp s n) = (val s ^ n) %% p.
-apply intind. progress. smt(@Zp).
+apply intind. progress. smt(@ZModpField @Sub).
 progress.
 rewrite exprSr. auto.
 rewrite ZModpField.exprSr. auto.
@@ -106,39 +105,107 @@ rewrite H0.
 smt(@IntDiv). 
 qed.
 
-lemma exps (x : zmod) : forall n, 0 <= n => (x ^ n)%Ring_ops_spec = (x ^^ n). 
+
+lemma exps (x : zmod) : forall n, 0 <= n => (x ^ n) = (x ^^ n). 
 apply intind. progress.
 smt(@Zp @Ring).
 progress.
-have ->: (x ^ (i + 1))%Ring_ops_spec = x * (x^ i)%Ring_ops_spec. 
+have ->: (x ^ (i + 1)) = x * (x^ i). 
  rewrite /(^).
  have ->: asint x ^ (i + 1) = (asint x) * (asint x ^ i). smt.
  rewrite inzmodM. congr. rewrite asintK. auto.
-have ->: (x ^^ (i + 1)) = x * (x^^i). smt.
+have ->: (x ^^ (i + 1)) = x * (x ^^ i). smt.
 rewrite H0.
 auto.
 qed.
 
-lemma rels_compat s w : (valR s) %% p <> 0 =>
- soundness_relationJ s w 
- =  LSP.soundness_relation  (ZPS.Sub.insubd (inzmod (valR s))) (LSP.EG.inzmod (valR w)).
-move => s_not_zero.
-rewrite /soundness_relationJ /soundness_relation /IsDL.
- have by_def: g = (inzmod g_int). admit. 
-rewrite by_def.
-rewrite exp_lemma5. rewrite - by_def. apply g_unit. smt(@W64xN).
-rewrite - by_def. rewrite g_q_assumption. auto.
-rewrite  lll. rewrite - by_def. apply g_unit.
-rewrite - bbb.
-rewrite ZPS.Sub.insubdK. rewrite /P. rewrite - by_def. smt(g_unit @ZModpField).
-rewrite ZPS.Sub.insubdK. rewrite /P. 
-apply unitE. rewrite /Zp.zero. smt(@Zp).
-have ->: (ZModpField.exp (inzmod g_int) (valR w)) = ((inzmod g_int) ^^ (valR w)). rewrite /(^^). auto.
+
+lemma completness_compat s w : 
+ completeness_relationJ s w
+ =  completeness_relationG (inzmod (valR s)) (valR w).
+(* move => s_not_zero. *)
+rewrite /completeness_relationJ /completeness_relation /IsDL.
+rewrite /completeness_relationG.
+have ->: (ZModpField.exp (inzmod Constants.g) (valR w)) = ((inzmod Constants.g)  ^^ (valR w)). auto.
 rewrite - exps. smt(@W64xN).
-rewrite /(^).
-rewrite inzmodK.
-have ->: (g_int %% p) = g_int. admit. (* by assumption *)
-smt.
+have ->: inzmod Constants.g ^ valR w = inzmod (Constants.g ^ valR w). smt.
+rewrite xxx. auto.
+qed.
+
+(* lemma rels_compat s w : (valR s) %% p <> 0 => *)
+(*  completeness_relationJ s w  *)
+(*  =  LSP.completeness_relation  (ZPS.Sub.insubd (inzmod (valR s))) (LSP.EG.inzmod (valR w)). *)
+(* move => s_not_zero. *)
+(* rewrite /completeness_relationJ /completeness_relation /IsDL. *)
+(* rewrite exp_lemma5. apply g_unit. smt(@W64xN). *)
+(* rewrite g_q_assumption. auto. *)
+(* rewrite  lll.  apply g_unit. *)
+(* rewrite - bbb. *)
+(* rewrite ZPS.Sub.insubdK. rewrite /P. smt(g_unit @ZModpField). *)
+(* rewrite ZPS.Sub.insubdK. rewrite /P.  *)
+(* apply unitE. rewrite /Zp.zero. smt(@Zp). *)
+(* have ->: (ZModpField.exp (inzmod Constants.g) (valR w)) = ((inzmod Constants.g) ^^ (valR w)). rewrite /(^^). auto. *)
+(* rewrite - exps. smt(@W64xN). *)
+(* rewrite /(^). *)
+(* rewrite inzmodK. *)
+(* have ->: (Constants.g %% p) = Constants.g. rewrite /Constants.g. smt(@Zp). *)
+(* rewrite xxx. *)
+(* have ->: (Constants.g %% Constants.p) = Constants.g. rewrite /Constants.g. smt(@Zp). *)
+(* auto. *)
+(* qed. *)
+
+(* TODO: move to constants *)
+op yy : int = 1619143025881598520624761283475402020548391884071535717508227364160250029021913075600233405069001566834683913353926864105451868045119367799203330594939018027579182910491986631752134379672737328627758392039634104925436356398864177945255144950961436710218515919232515425511046597212472673535352725377222373577674557399263766126616709301502213900518108948863077641585338203695018313411734375313490314236425883902205676609966518701386913481608853106992344785426585987776048274548105346527876890352239772208848767741675883443476938540148618750188887210747096545526357760228916139597422735471808664106841641302833036768868.
+
+op zz : int = 32317006071311007301090839450916075672074637894498330470309491614874605269258845429066617750438611497217172998255766216223761011478474532650974905473458381524348224983452534238842699055706528839316900073176359409123413739445397952234623184300460154670470987008412185029124584489601900670931121854398190604800292822877845957165654247519063010445688374293905515743037557007239230573090162415731314434935337651887720640264611889321352234483385341531370885728478742938129783934088697644527630028295616871380503535956364143710134154492766231832072494607343336005619107670188720508364918065676485338559326165037076233303652.
+
+op ww : int = 1044388881413152506691752710716624382579964249047383780384233483283953907971557456848826811934997558340890106714439262837987573438185793607263236087851365277945956976543709998340361590134383718314428070011855946226376318839397712745672334684344586617496807908705803704071284048740118609114467977783598029006686938976881787785946905630190260940599579453432823469303026696443059025015972399867714215541693835559885291486318237914434496734087811872639496475100189041349008417061675093668333850551032972088269550769983616369411933015213796825837188091833656751221318492846368125550225998300412344784862595674492194617023806505913245610825731835380087608622102834270197698202313169017678006675195485079921636419370285375124784014907159135459982790513399611551794271106831134090584272884279791554849782954323534517065223269061394905987693002122963395687782878948440616007412945674919823050571642377154816321380631045902916136926708342856440730447899971901781465763473223850267253059899795996090799469201774624817718449867455659250178329070473119433165550807568221846571746373296884912819520317457002440926616910874148385078411929804522981857338977648103126085903001302413467189726673216491511131602920781738033436090243804708340403154190336.
+
+
+lemma pq_euclid : euclidef ww Constants.p (zz, yy).
+rewrite /euclidef. split. auto.
+smt().
+qed.
+
+
+lemma bp_comp : Ri = Constants.bp. 
+rewrite /Ri. rewrite nasty_id. simplify.
+rewrite /edivz. simplify. simplify.
+have ->: `|Constants.p| = Constants.p. 
+auto.
+rewrite /edivn. simplify. rewrite /euclidef. simplify.
+have ->: Constants.p < 0 = false. auto. simplify.
+have ->: (Constants.p = 0) = false. auto. simplify.
+pose P := (fun (qr : int * int) =>
+        ww =
+        qr.`1 * Constants.p + qr.`2 /\ 0 <= qr.`2 && qr.`2 < `|Constants.p|).
+have f1 : P (choiceb P (0,0)).
+apply choicebP. exists (zz,yy). rewrite /P. simplify. split. rewrite /ww /zz /Constants.p /yy. simplify. auto.
+smt(). 
+elim f1. 
+have z: choiceb
+     (fun (qr : int * int) =>
+        ww =
+        qr.`1 * Constants.p + qr.`2 /\ 0 <= qr.`2 && qr.`2 < `|Constants.p|) (0,0) 
+  = (choiceb P (0, 0)). auto.
+progress. rewrite z.
+rewrite /signz. 
+have ->: (Constants.p < 0) = false. auto. simplify.
+have ->: (Constants.p <> 0) = true. auto. 
+have ->: (-1) ^ b2i false = 1. rewrite /b2i. simplify. auto.
+have ->: 1 * b2i true  = 1. rewrite /b2i. simplify.  auto. simplify.
+have ->: (let (q, r) = choiceb P (0, 0) in (q, r)).`1 = (choiceb P (0, 0)).`1.  smt().
+have mem' : 
+  forall (x1 y1 x2 y2 l : int),
+    x1 \in range 0 l =>
+    x2 \in range 0 l => x1 + l * y1 = x2 + l * y2 => y1 = y2 .
+smt(mem_range_add_mul_eq).
+have : (choiceb P (0, 0)).`1 = zz.
+apply (mem' (choiceb P (0, 0)).`2 (choiceb P (0, 0)).`1  yy zz  Constants.p). 
+smt(@List). smt(@List).
+have ->: (choiceb P (0, 0)).`2 + Constants.p * (choiceb P (0, 0)).`1 = (choiceb P (0, 0)).`1 * Constants.p + (choiceb P (0, 0)).`2.
+smt().
+rewrite - H. simplify. rewrite /ww /yy /zz /Constants.p. simplify. done.  auto.
 qed.
 
 
@@ -161,14 +228,14 @@ ecall {2} (bnreduce_small_spec_ph response_0{2} exp_order{2}). simplify.
 ecall {2} (bnreduce_small_spec_ph challenge_0{2} exp_order{2}). simplify.
 ecall {2} (bnreduce_small_spec_ph commitment_0{2} group_order{2}). simplify.
 ecall {2} (bnreduce_small_spec_ph statement{2} group_order{2}). simplify.
-call{2} bn_set_gg_prop.
-call{2} bn_set_bf_prop.
-call{2} bn_set_go_prop.
-call{2} bn_set_eb_prop.
-call{2} bn_set_eo_prop.
+call{2} Constants.bn_set_g_correct.
+call{2} Constants.bn_set_bp_correct.
+call{2} Constants.bn_set_p_correct.
+call{2} Constants.bn_set_bq_correct.
+call{2} Constants.bn_set_q_correct.
 simplify.
 skip. progress.
-rewrite ri_un. rewrite H6. rewrite Ri_def. rewrite /ri. smt().
+rewrite ri_un. rewrite H6. rewrite /ri. smt().
 rewrite H5. smt(prime_p).
 smt(@W64xN).
 smt(@W64xN).
@@ -179,7 +246,7 @@ smt(@W64xN).
 smt(@W64xN).
 rewrite H5. 
 smt(p_val_prop1).
-rewrite ri_un. rewrite H4. rewrite Rip_def. rewrite /ri. rewrite H3. smt().
+rewrite ri_un. rewrite H4. rewrite /ri. rewrite H3. smt().
 smt(q_prime).
 smt(@W64xN).
 smt(@W64xN).
@@ -189,7 +256,9 @@ smt(@W64xN).
 smt(@W64xN).
 smt(q_val_prop1).
 smt().
-rewrite /R. rewrite - H6.  
+rewrite /R. 
+rewrite bp_comp.
+rewrite - H6.  
 rewrite R2.bnK. auto.
 smt(@W64xN).
 smt().
@@ -198,7 +267,8 @@ smt().
 smt(@Zp).
   have sq_fact: ((ZModpField.exp s{1} q) = ZPS.Zp.one)
             = (result15 = W64.one). 
-  rewrite H58 H56 H15 H5 H3 H57 - H.
+  rewrite H58. rewrite H56. rewrite H15. rewrite H5. rewrite H3. rewrite H57.
+  have ->: (valR statement{2} %% Constants.p) = val s{1}. smt().
   have ->: (ZModpField.exp s{1} q) = s{1} ^^ q. 
     rewrite /(^^). smt(@ZModpField).
     rewrite - exps. smt(q_prime). rewrite /(^) /asint /ZPS.Zp.one xxx.  
@@ -223,19 +293,20 @@ rewrite exps_same. auto.
 have  <- : (ZModpField.exp s{1} (c{1} %% q)) = (ZModpField.exp s{1} c{1}). 
 rewrite (exp_mod s{1} c{1} q). rewrite sq_fact. auto. auto.
 rewrite exps'. smt(@IntDiv).
-auto.
+auto. auto.
 rewrite /(^).
-have ->: val (g ^^ t{1})  = val (g ^^ (t{1} %% q)).
-rewrite /(^^). rewrite - exps_same.
+have ->: val (ZModpField.exp g t{1})  = val (ZModpField.exp g (t{1} %% q)).
+rewrite /(^^).
 rewrite (exp_mod g t{1} q). rewrite g_q_assumption. auto.
 auto.
-rewrite - exps'. smt(@IntDiv). rewrite /(^^). rewrite exps_same. auto.
+rewrite  exps'. smt(@IntDiv). auto. rewrite /Constants.g /g. smt(@Zp).
 progress.
 rewrite (w64_and result12 result15). smt(). smt().
 rewrite (w64_and_false result12 result15). 
 smt(). smt().
 smt().
 qed.
+
 
 require import UniformSampling_Concrete.
 
@@ -249,19 +320,19 @@ symmetry. call expm_correct.
 symmetry.
 call usample_aspec. sp.
 simplify.
-call{1} bn_set_bf_prop.
-call{1} bn_set_gg_prop.
-call{1} bn_set_go_prop.
-call{1} bn_set_eo_prop.
+call{1} Constants.bn_set_bp_correct.
+call{1} Constants.bn_set_g_correct.
+call{1} Constants.bn_set_p_correct.
+call{1} Constants.bn_set_q_correct.
 skip. move => &1 _ H r qe r2 vr rr iz rp vri.
 split. rewrite qe. simplify. smt(q_prime).
 move => h1. move => rL rR. move => rzrlrr. 
 split. 
-split.  smt. split. smt. split.  smt. split.  smt. rewrite /R. rewrite - vri. smt(@W64x2N @R2).
+split.  smt. split. smt. split.  smt. split.  smt. rewrite /R. 
+rewrite bp_comp.
+rewrite - vri. smt(@W64x2N @R2).
 move => qo. move => rl rrr ai. smt.
 qed.
-
-
 
 
 lemma commit_same : 
@@ -312,11 +383,8 @@ transitivity ASpecFp_Schnorr.challenge
 apply challenge_same.
 proc. 
 symmetry. call usample_aspec.
-call{1} bn_set_eo_prop. wp. skip. progress.
-smt.
+call{1} Constants.bn_set_q_correct. wp. skip. progress.
 qed.
-
-
 
 
 lemma response_eq : 
@@ -331,11 +399,11 @@ ecall {2} (bn_mulm_correct challenge_0{2} witness0{2} exp_order{2}). simplify.
 ecall {2} (bnreduce_small_spec_ph witness0{2} exp_order{2}). simplify.
 ecall {2} (bnreduce_small_spec_ph secret_power{2} exp_order{2}). simplify.
 ecall {2} (bnreduce_small_spec_ph challenge_0{2} exp_order{2}). simplify.
-call{2} bn_set_eb_prop. simplify.
-call{2} bn_set_eo_prop. simplify.
+call{2} Constants.bn_set_bq_correct. simplify.
+call{2} Constants.bn_set_q_correct. simplify.
 wp.
 skip. 
-progress. rewrite H3. rewrite Rip_def. rewrite ri_un. rewrite /ri. rewrite H2. smt().
+progress. rewrite H3. rewrite ri_un. rewrite /ri. rewrite H2. smt().
 smt. 
 smt(@W64xN).
 smt(@W64xN).
