proof/schnorr_protocol/W64_SchnorrCompleteness.ec
@@ -3,12 +3,15 @@ require import AllCore Distr DInterval List Int IntDiv.
 from Jasmin require import JModel JBigNum.
 require import Array32 Array64 Array128.
 
-require import Zp_SchnorrProtocol.
 require import W64_SchnorrProtocol.
-require import W64_Zp_SchnorrIndistinguishability.
 require import Ring_ops_spec.
-import Zp DZmodP.
-import W64xN Sub R. 
+(* import Zp DZmodP  Sub . *)
+
+import W64xN. 
+
+require import W64_Zp_SchnorrIndistinguishability.
+import ZPSP.
+import Zp.
 
 module CompletenessJ(P:ZKProverJ,V:ZKVerifierJ) = {
   proc main(s:W64.t Array32.t, w:W64.t Array32.t) = {
@@ -22,8 +25,8 @@ module CompletenessJ(P:ZKProverJ,V:ZKVerifierJ) = {
 }.
 
 
-lemma completeness ss ww &m:
- Pr[ CompletenessG(SchnorrProver,SchnorrVerifier).main(inzmod (W64xN.valR ss) , (W64xN.valR ww))@&m : res]
+lemma completeness_same ss ww &m:
+ Pr[ CompletenessG(SchnorrProver,SchnorrVerifier).main(ZPSP.Zp.inzmod (W64xN.valR ss) , (W64xN.valR ww))@&m : res]
  = Pr[CompletenessJ(JProver,JVerifier).main(ss,ww)@&m : res].
 proof.
 byequiv.
@@ -34,11 +37,44 @@ call challenge_eq.
 call commitment_eq.
 simplify. skip. progress.
 smt. smt. rewrite H. 
-have v : valR result_R.`1 < p. rewrite - H. smt(@Zp).
-have : valR result_R.`1 %% p = valR result_R.`1. smt (@IntDiv @Zp).
+have v : valR result_R.`1 < ZPSP.Zp.p. rewrite - H. smt(@Zp).
+have : valR result_R.`1 %% ZPSP.Zp.p = valR result_R.`1. smt (@IntDiv @Zp).
 smt().
 rewrite - H2.
 smt.
 smt.
 auto. auto.
+qed.
+
+import MLC.
+lemma qqqq x : 0 <= x => (Constants.g ^ x %% Zp.p) <> 0.
+move => xnonzero.
+case ((Constants.g ^ x %% Zp.p = 0)).
+move => q. simplify.
+  have : unit (ZModpField.exp g x ).
+  smt.
+rewrite /unit. elim. 
+move => y.
+have : Sub.val (y * (ZModpField.exp g x) )= ((Sub.val y) * (Sub.val (ZModpField.exp g x)) %% Zp.p). 
+smt.
+have ->: (Sub.val ((ZModpField.exp g x))) = ((Sub.val g) ^ x) %% p.
+ have -> : (ZModpField.exp g x) = g ^^ x. auto.
+rewrite  - exps. assumption.
+smt.
+move => eq1 eq2.
+have o1 : (Sub.val y) * ((Sub.val g) ^ x %% p) %% Zp.p = 0.
+  have -> : (Sub.val g) = Constants.g. smt(@Sub). rewrite q. simplify. auto.
+have o2 : (Sub.val y) * ((Sub.val g) ^ x %% p) %% Zp.p = 1.
+ rewrite - eq1. rewrite eq2. smt(@Sub).
+smt().
+auto.
+qed.
+
+
+lemma completenessJ ss ww &m: completeness_relationJ ss ww =>
+ Pr[CompletenessJ(JProver,JVerifier).main(ss,ww)@&m : res] = 1%r.
+move => compl_rel.
+rewrite - completeness_same.
+apply  (ZPSP.completenessG (ZPSP.Zp.inzmod (W64xN.valR ss)) (W64xN.valR ww) &m).
+rewrite - (completness_compat ss ww). auto. 
 qed.
